Trying stuff

Map.v
@@ -18,7 +18,9 @@ Definition lookup {A : Type} (m : map A) k := m k.
 
 Notation "m '[' k '<==' v ']'" := (update m k v) (at level 9).
 
-(* Proofs *)
+(* ------------------------------------------------------------------------- *)
+(* Proofs                                                                    *)
+(* ------------------------------------------------------------------------- *)
 
 Lemma lookup_update_eq : forall {A} (m : map A) k v,
   m[k <== v] k = Some v.
@@ -36,20 +38,69 @@ Proof.
   apply eqb_eq in E. contradiction.
 Qed.
 
+(* ------------------------------------------------------------------------- *)
+(* Equivalence                                                               *)
+(* ------------------------------------------------------------------------- *)
+
+Definition equivalent {A} (m1 m2 : map A) :=
+  forall k, m1 k = m2 k.
+
+Lemma equivalent_refl : forall {A} (m1 m2 : map A),
+  equivalent m1 m2 ->
+  equivalent m2 m1.
+Proof.
+  unfold equivalent in *. intros. eauto.
+Qed.
+
+Lemma equivalent_lookup : forall {A} (m1 m2 : map A) k v,
+  equivalent m1 m2 ->
+  m1 k = v ->
+  m2 k = v. 
+Proof.
+  intros * Heq ?. specialize (Heq k). inversion Heq. trivial.
+Qed.
+
+Lemma equivalent_update : forall {A} (m1 m2 : map A) k v,
+  equivalent m1 m2 ->
+  equivalent m1[k <== v] m2[k <== v].
+Proof.
+  unfold equivalent, update, update'. intros. destruct eqb; eauto.
+Qed.
+
+Lemma equivalent_update_permutation : forall {A} (m : map A) k1 k2 v1 v2,
+  k1 <> k2 ->
+  equivalent m[k1 <== v1][k2 <== v2] m[k2 <== v2][k1 <== v1].
+Proof.
+  unfold equivalent, update, update'. intros.
+  destruct (eqb k1 k) eqn:E1; destruct (eqb k2 k) eqn:E2; auto.
+  apply eqb_eq in E1, E2. subst. contradiction.
+Qed.
+
+Lemma equivalent_update_overwrite : forall {A} (m : map A) k v v',
+  equivalent m[k <== v] m[k <== v'][k <== v].
+Proof.
+  unfold equivalent, update, update'. intros.
+  destruct eqb; intros; trivial.
+Qed.
+
+(* ------------------------------------------------------------------------- *)
+(* Inclusion                                                                 *)
+(* ------------------------------------------------------------------------- *)
+
 (* m includes m' *)
 Definition includes' {A} (m m' : map A) := forall k v,
   m' k = Some v -> m k = Some v.
 
 Infix "includes" := includes' (at level 50, left associativity).
 
-Lemma update_preserves_inclusion : forall {A} (m m' : map A) k v,
+Lemma inclusion_update : forall {A} (m m' : map A) k v,
   m includes m' ->
   m[k <== v] includes m'[k <== v].
 Proof.
   unfold includes', update, update'. intros. destruct eqb; auto.
 Qed.
 
-Lemma update_permutation : forall {A} (m : map A) k1 k2 v1 v2,
+Lemma inclusion_update_permutation : forall {A} (m : map A) k1 k2 v1 v2,
   k1 <> k2 ->
   m[k1 <== v1][k2 <== v2] includes m[k2 <== v2][k1 <== v1].
 Proof.
@@ -58,25 +109,10 @@ Proof.
   apply eqb_eq in E1, E2. subst. contradiction.
 Qed.
 
-Lemma update_permutation' : forall {A} (m : map A) k k1 k2 v1 v2,
-  k1 <> k2 ->
-  m[k1 <== v1][k2 <== v2] k = m[k2 <== v2][k1 <== v1] k.
-Proof.
-  unfold includes', update, update'. intros.
-  destruct (eqb k1 k) eqn:E1; destruct (eqb k2 k) eqn:E2; auto.
-  apply eqb_eq in E1, E2. subst. contradiction.
-Qed.
-
-Lemma update_overwrite : forall {A} (m : map A) k v v',
+Lemma inclusion_update_overwrite : forall {A} (m : map A) k v v',
   m[k <== v] includes m[k <== v'][k <== v].
 Proof.
   unfold includes', update, update'. intros.
   destruct eqb; intros; assumption.
 Qed.
 
-Lemma update_overwrite' : forall {A} (m : map A) k k' v v',
-  m[k' <== v] k = m[k' <== v'][k' <== v] k.
-Proof.
-  unfold includes', update, update'. intros.
-  destruct eqb; intros; trivial.
-Qed.
